wip : how to execute module?

extract/bin/main.ml
@@ -1,0 +1,49 @@
+open Stdlib
+
+open Coq_extracted
+open ITreeDefinition
+open Events
+open Datatypes
+open Any
+
+let rec to_int = function | O -> 0 | S n -> succ (to_int n)
+let rec of_int n = assert(n >= 0); if(n == 0) then O else S (of_int (pred n))
+
+let string_of_nat n =
+  string_of_int (to_int n)
+
+let string_of_ret a =
+  match (Any.downcast a) with
+  | Some n -> string_of_nat n
+  | None -> raise (Failure "return value is not natural number")
+
+let handle_Event = fun e k ->
+  match e with
+  | Choose -> raise (Failure "nondeterminism(choose) error")
+  | Take -> raise (Failure "nondeterminism(take) error")
+  | IO (str, arg) -> 
+    match str with
+    | "dprint" -> print_endline ("Debug : " ^ (Obj.obj arg)); k (Obj.repr ())
+    | "choose_index" -> 
+      let n = List.length (Obj.obj arg) in
+      let idx = Random.int n in
+      k (Obj.repr (of_int idx))
+    | "choose_optbool" -> 
+      let random_optbool =
+        match Random.int 3 with
+        | 0 -> None
+        | 1 -> Some false
+        | _ -> Some true in
+      k (Obj.repr random_optbool)
+    | _ -> raise (Failure "system call error")
+
+let rec run t =
+  match observe t with
+  | RetF r -> print_endline ("Return : " ^ (string_of_ret r))
+  | TauF t -> run t
+  | VisF (e, k) -> handle_Event e (fun x -> run (k x))
+
+let main =
+  print_endline "start test";
+  Random.self_init ();
+  run (Example0.ttitr)
