extract/extraction.v
@@ -1,27 +1,46 @@
-(* Require Import ImpPrelude.
-Require Import ModSem.
+Require Extraction.
+Require Import ExtrOcamlBasic.
+Require Import ExtrOcamlNativeString.
+
+From ITree Require Import ITreeDefinition.
 Require Import ClassicalDescription.
 
-Require Coq.extraction.Extraction.
-Require Import ExtrOcamlBasic.
-Require Import ExtrOcamlString.
-(* Require Import Coq.extraction.ExtrOcamlZInt. *)
-(* Require Import ExtrOcamlNatInt. *)
+Require Import SchI SchHeader.
+
+Set Extraction Output Directory "extract/coq_extracted".
 
 Extraction Blacklist List String Int.
 
 Extract Constant excluded_middle_informative => "true".
-Extract Constant assume => "(fun _ -> lazy (Coq_go (RetF ())))".
-Extract Constant guarantee => "(fun _ -> lazy (Coq_go (RetF ())))".
 
-Require Import Imp ImpNotations lm_main.
-        (* EchoAll *)
+Extract Constant SchI.choose_index =>
+   "fun _ tids ->
+      ITree.bind
+        (ITree.trigger
+          (subevent
+            (coq_ReSum_inr (Obj.magic __) (fun _ _ _ x x0 _ ->
+              coq_Cat_IFun x x0) (fun _ _ _ -> coq_Inr_sum1) __ __ __
+              (coq_ReSum_inr (Obj.magic __) (fun _ _ _ x x0 _ ->
+                coq_Cat_IFun x x0) (fun _ _ _ -> coq_Inr_sum1) __ __ __
+                (coq_ReSum_inr (Obj.magic __) (fun _ _ _ x x0 _ ->
+                  coq_Cat_IFun x x0) (fun _ _ _ -> coq_Inr_sum1) __ __ __
+                  (coq_ReSum_id (fun _ _ -> coq_Id_IFun) __)))) 
+            (IO (""choose_index"", (Obj.magic tids))))) 
+      (fun x_ -> lazy (Coq_go (RetF x_)))".
 
-Cd "extract".
+Extract Constant Sch.yield =>
+   "fun h h0 ->
+      Seal.sealing coq_SCH
+      (iterC (fun _ ->
+        ITree.bind (ITree.trigger (subevent h (IO (""choose_optbool"", (Obj.magic ()))))) (fun b ->
+          match b with
+          | Some y ->
+            if y
+            then ITree.bind
+                   (ITree.trigger
+                     (subevent h0 (Call (SchHdr.yield, (Any.Any.upcast ())))))
+                   (fun _ -> lazy (Coq_go (RetF (Coq_inl ()))))
+            else lazy (Coq_go (RetF (Coq_inl ())))
+          | None -> lazy (Coq_go (RetF (Coq_inr ()))))) ())".
 
-Separate Extraction Z.to_nat Z.opp lm_main.test_itr
-         (* mw_impl_itr mw_abs_itr EXTRACT_MW_IMPL_LINKING_CHECK *)
-.
-         (* echo_prog *)
-
-Cd "..". *)
+(* Separate Extraction observe ttitr. *)
